A not unsuccessful refactoring of BSTs and the Set interface.

DS/BST2.v
@@ -2,33 +2,14 @@ Require Import BTree.
 Require Export LinDec.
 Require Import Sorting.Sort.
 
-(*
-Require Import ssreflect.
-*)
-
-Check compare.
-Print comparison.
-Search comparison.
-Print CompareSpec.
-Search compare.
-Print compare.
-
 Inductive isBST
-  {A : Type} {cmp : A -> A -> comparison} : BTree A -> Type :=
+  {A : Type} {cmp : A -> A -> comparison} : BTree A -> Prop :=
     | isBST_empty : isBST empty
-    | isBST_node_l :
-        forall (v x : A) (ll lr : BTree A),
-          isBST (node x ll lr) -> cmp x v = Lt ->
-            isBST (node v (node x ll lr) empty)
-    | isBST_node_r :
-        forall (v x : A) (rl rr : BTree A),
-          isBST (node x rl rr) -> cmp x v = Gt ->
-            isBST (node v empty (node x rl rr))
-    | isBST_node_lr :
-        forall (v xl xr : A) (ll lr rl rr : BTree A),
-          isBST (node xl ll lr) -> cmp xl v = Lt ->
-          isBST (node xr rl rr) -> cmp xr v = Gt ->
-            isBST (node v (node xl ll lr) (node xr rl rr)).
+    | isBST_node :
+        forall (v : A) (l r : BTree A),
+          isBST l -> (forall x : A, elem x l -> cmp x v = Lt) ->
+          isBST r -> (forall x : A, elem x r -> cmp x v = Gt) ->
+            isBST (node v l r).
 
 Arguments isBST {A} _ _.
 
@@ -40,7 +21,7 @@ Record BST {A : Type} (cmp : A -> A -> comparison) : Type :=
     prop : isBST cmp tree
 }.
 
-Fixpoint elem_dec
+Function elem_dec
   {A : Type} (cmp : A -> A -> comparison) (x : A) (t : BTree A) : bool :=
 match t with
     | empty => false
@@ -52,48 +33,18 @@ match t with
         end
 end.
 
-Lemma elem_dec_spec :
-  forall {A : Type} (cmp : A -> A -> comparison) (x : A) (t : BTree A),
-    (forall x y : A, CompareSpec (x = y) (cmp x y = Lt) (cmp x y = Gt) (cmp x y)) ->
-      isBST cmp t -> BoolSpec (elem x t) (~ elem x t) (elem_dec cmp x t).
-Proof.
-  intros A cmp x t spec H.
-  revert t H.
-  induction t; intros; cbn.
-    constructor. inversion 1.
-    destruct (spec x a); subst.
-      constructor. constructor.
-      destruct IHt1.
-        admit.
-        do 2 constructor. assumption.
-        constructor. inversion 1; subst.
-          Search CompareSpec.
-Abort.
-
-Fixpoint BTree_ins
+Function insert
   {A : Type} (cmp : A -> A -> comparison)
   (x : A) (t : BTree A) : BTree A :=
 match t with
     | empty => node x empty empty
     | node v l r =>
         match cmp x v with
-            | Lt => node v (BTree_ins cmp x l) r
+            | Lt => node v (insert cmp x l) r
             | Eq => node x l r
-            | Gt => node v l (BTree_ins cmp x r)
+            | Gt => node v l (insert cmp x r)
         end
 end.
-
-(*
-Lemma elem_ins : forall (A : LinDec) (x a : A) (t : BTree A),
-    elem x (BTree_ins a t) -> x = a \/ elem x t.
-Proof.
-  move=> A x a t. elim: t => [| v l Hl r Hr] //=.
-    inv 1.
-    dec; inv H.
-      case: Hl; auto.
-      case: Hr; auto.
-Qed.
-*)
 
 Fixpoint min {A : Type} (t : BTree A) : option A :=
 match t with
@@ -103,9 +54,95 @@ match t with
 end.
 
 (** [fromList] and its variants. *)
-(*Function fromList (A : LinDec) (l : list A) : BTree A :=
+Fixpoint fromList
+  {A : Type} (cmp : A -> A -> comparison) (l : list A) : BTree A :=
 match l with
     | [] => empty
-    | h :: t => BTree_ins h (fromList A t)
+    | h :: t => insert cmp h (fromList cmp t)
 end.
-*)
+
+Function removeMin
+  {A : Type} (cmp : A -> A -> comparison)
+  (t : BTree A) : option (A * BTree A) :=
+match t with
+    | empty => None
+    | node x l r =>
+        match removeMin cmp l with
+            | None => Some (x, r)
+            | Some (m, l') => Some (m, node x l' r)
+        end
+end.
+
+Function BST_remove
+  {A : Type} (cmp : A -> A -> comparison)
+  (x : A) (t : BTree A) : BTree A :=
+match t with
+    | empty => empty
+    | node v l r =>
+        match cmp x v with
+            | Lt => node v (BST_remove cmp x l) r
+            | Gt => node v l (BST_remove cmp x r)
+            | Eq =>
+                match removeMin cmp l with
+                    | None => r
+                    | Some (m, l') => node m l' r
+                end
+        end
+end.
+
+Lemma elem_dec_spec :
+  forall {A : Type} (cmp : A -> A -> comparison) (x : A) (t : BTree A),
+    (forall x y : A, CompareSpec (x = y) (cmp x y = Lt) (cmp x y = Gt) (cmp x y)) ->
+      isBST cmp t -> BoolSpec (elem x t) (~ elem x t) (elem_dec cmp x t).
+Proof.
+  intros A cmp x t spec H.
+  functional induction (elem_dec cmp x t).
+    constructor. inversion 1.
+    inversion H; subst. specialize (IHb H3). destruct IHb.
+      constructor. constructor 2. assumption.
+      constructor. inversion 1; subst.
+        admit.
+        contradiction.
+        specialize (H6 _ H7). congruence.
+    constructor. destruct (spec x v); try congruence; subst. constructor.
+    inversion H; subst. specialize (IHb H5). destruct IHb.
+      constructor. constructor 3. assumption.
+      constructor. inversion 1; subst.
+        admit.
+        specialize (H4 _ H7). congruence.
+        contradiction.
+Admitted.
+
+Lemma elem_insert :
+  forall {A : Type} (cmp : A -> A -> comparison) (x : A) (t : BTree A),
+    isBST cmp t -> elem_dec cmp x (insert cmp x t) = true.
+Proof.
+  intros.
+  functional induction (insert cmp x t); cbn.
+    admit.
+    rewrite e0, IHb.
+      reflexivity.
+      inversion H; assumption.
+    admit.
+    rewrite e0, IHb.
+      reflexivity.
+      inversion H; assumption.
+Admitted.
+
+Lemma elem_remove :
+  forall (A : Type) (cmp : A -> A -> comparison) (x : A) (t : BTree A),
+    isBST cmp t -> elem_dec cmp x (BST_remove cmp x t) = false.
+Proof.
+  intros.
+  functional induction (BST_remove cmp x t); cbn.
+    reflexivity.
+    rewrite e0, IHb.
+      reflexivity.
+      inversion H; assumption.
+    rewrite e0, IHb.
+      reflexivity.
+      inversion H; assumption.
+    inversion H; subst.
+      admit.
+Abort.
+
