ADT/FinSet2.v
@@ -1,0 +1,44 @@
+Require Import RCCBase.
+
+Module Type FinSet.
+
+Parameters E S : Type.
+
+Parameter empty : S.
+
+Parameter insert : E -> S -> S.
+
+Parameter remove : E -> S -> S.
+
+Parameter isEmpty : S -> bool.
+
+Parameter member : E -> S -> bool.
+
+(** Properties of [member]. *)
+
+Parameter member_insert :
+  forall (x : E) (s : S),
+    member x (insert x s) = true.
+
+Parameter member_remove :
+  forall (x : E) (s : S),
+    member x (remove x s) = false.
+
+Parameter member_insert' :
+  forall (x y : E) (s : S),
+    x <> y -> member x (insert y s) = member x s.
+
+Parameter member_remove' :
+  forall (x y : E) (s : S),
+    x <> y -> member x (remove y s) = member x s.
+
+(** Definition of equivalent sets. *)
+
+Definition equiv (s1 s2 : S) : Prop :=
+  forall x : E, member x s1 = member x s2.
+
+Parameter remove_insert_equiv :
+  forall (x : E) (s : S),
+    equiv (remove x (insert x s)) s.
+
+End FinSet.
