ADT/Queue.v
@@ -1,5 +1,3 @@
-
-
 Require Import RCCBase.
 
 Module Type Queue.
